secure_api/uf1cma/Crypto.Symmetric.MAC.fst
@@ -185,7 +185,7 @@ let frame_sel_elem h1 h2 #i b =
 
 #reset-options "--z3rlimit 50 --initial_fuel 0 --max_fuel 0 --max_ifuel 1 --initial_ifuel 1"
 (** Create and initialize an element (used for r) *)
-val rcreate: rgn:HS.rid{HS.is_eternal_region rgn} -> i:id -> ST (elemB i)
+val rcreate: rgn:HS.rid{is_eternal_region rgn} -> i:id -> ST (elemB i)
   (requires (fun h0 -> True))
   (ensures  (fun h0 r h1 ->
     HS.modifies (Set.singleton rgn) h0 h1 /\
